Change the order required on the elements
This commit cleans loosen the constraints the comparison operator that compares the elements in the priority queue. This was necessary because when we will have to prove the correctness of the delete operation, we will need the fact that an ordered boostraped heap stores its children in an ordered skew binomial heap.
To prove that merge and insert preserve this ordering, we needed to prove that b_comparison_heap (a function that creates a comparator between bootstraped heaps from a comparison between elements) maintains the weak linearity of the relation.
This was not possible so I switched to a total pre-order, which turns out to be enough.

translator/okasaki-examples/SkewBinomialHeapScript.sml
@@ -162,7 +162,9 @@ val b_is_empty_def = Define `
 Create a comparison function for bootstraped binomial heaps
 from a comparison function for their roots
 *)
-val b_heap_comparison = Define `
+val b_heap_comparison_def = Define `
+  (b_heap_comparison geq Bsbempty _ = T) /\
+  (b_heap_comparison geq _ Bsbempty = F) /\
   (b_heap_comparison geq (Bsbheap r1 _) (Bsbheap r2 _) = geq r1 r2)
 `;
 
@@ -211,6 +213,7 @@ val b_heap_to_bag_def = Define `
 val is_b_heap_ordered_def = Define `
   (is_b_heap_ordered geq Bsbempty = T) /\
   (is_b_heap_ordered geq (Bsbheap r c) = ((BAG_EVERY (\y. geq y r) (b_heap_to_bag1 geq c)) /\
+                                          (is_heap_ordered (b_heap_comparison geq) c) /\
                                           (is_b_heap_ordered1 geq c))) /\
   (is_b_heap_ordered1 geq [] = T) /\
   (is_b_heap_ordered1 geq (t::ts) = (is_b_heap_ordered2 geq t /\ is_b_heap_ordered1 geq ts)) /\
@@ -220,6 +223,11 @@ val is_b_heap_ordered_def = Define `
   (is_b_heap_ordered3 geq (e::es) = (is_b_heap_ordered geq e /\ is_b_heap_ordered3 geq es)) /\
   (is_b_heap_ordered4 geq [] = T) /\
   (is_b_heap_ordered4 geq (t::ts) = (is_b_heap_ordered2 geq t /\ is_b_heap_ordered4 geq ts))
+`;
+
+(* Requirements for the relation between elements *)
+val TotalPreOrder = Define `
+  TotalPreOrder R = (PreOrder R /\ total R)
 `;
 
 (* Useful lemmas *)
@@ -241,13 +249,13 @@ Proof
 QED;
 
 Theorem root_smallest:
-  !geq t y. WeakLinearOrder geq /\
+  !geq t y. TotalPreOrder geq /\
             is_tree_ordered geq t /\
             BAG_IN y (tree_to_bag t)==>
             geq y (root t)
 Proof
   rpt strip_tac \\
-  fs[WeakLinearOrder, WeakOrder] \\
+  fs[TotalPreOrder, PreOrder] \\
   Cases_on `t` \\
   Induct_on `l` \\
   rw[is_tree_ordered_def, tree_to_bag_def, root_def, BAG_EVERY] \\
@@ -256,8 +264,7 @@ Proof
 QED;
 
 Theorem children_order:
-  !geq t. WeakLinearOrder geq /\
-          is_tree_ordered geq t ==>
+  !geq t. is_tree_ordered geq t ==>
           is_heap_ordered geq (children t)
 Proof
   rpt strip_tac \\
@@ -267,8 +274,7 @@ Proof
 QED;
 
 Theorem app_heap_order:
-  !geq h1 h2. WeakLinearOrder geq /\
-              is_heap_ordered geq h1 /\
+  !geq h1 h2. is_heap_ordered geq h1 /\
               is_heap_ordered geq h2 ==>
               is_heap_ordered geq (APPEND h1 h2)
 Proof
@@ -278,8 +284,7 @@ Proof
 QED;
 
 Theorem reverse_heap_order:
-  !geq h. WeakLinearOrder geq /\
-          is_heap_ordered geq h ==>
+  !geq h. is_heap_ordered geq h ==>
           is_heap_ordered geq (REVERSE h)
 Proof
   rpt strip_tac \\
@@ -334,6 +339,32 @@ Proof
   rw[merge_def, normalize_def, merge_tree_def]
 QED;
 
+Theorem b_comparison_total_pre_order:
+  !geq. TotalPreOrder geq ==> TotalPreOrder (b_heap_comparison geq)
+Proof
+  rw[TotalPreOrder, PreOrder, reflexive_def,
+     transitive_def, total_def]
+  >- (Cases_on `x`
+      >- rw[b_heap_comparison_def]
+      >- rw[b_heap_comparison_def])
+  >- (Cases_on `x` \\ Cases_on `z`
+      >- rw[b_heap_comparison_def]
+      >- rw[b_heap_comparison_def]
+      >- (Cases_on `y`
+          >- rw[]
+          >- fs[b_heap_comparison_def])
+      >- (rw[b_heap_comparison_def] \\
+          Cases_on `y`
+          >- fs[b_heap_comparison_def]
+	  >- (fs[b_heap_comparison_def] \\
+              metis_tac[transitive_def])))
+  >- (Cases_on `x` \\ Cases_on `y`
+      >- (DISJ1_TAC \\ rw[b_heap_comparison_def])
+      >- (DISJ1_TAC \\ rw[b_heap_comparison_def])
+      >- (DISJ2_TAC \\ rw[b_heap_comparison_def])
+      >- (rw[b_heap_comparison_def]))
+QED;
+
 (* For both kinds of links, linking preserve the elements in the trees *)
 Theorem tree_link_bag:
   !geq t1 t2. tree_to_bag (tree_link geq t1 t2) = BAG_UNION (tree_to_bag t1) (tree_to_bag t2)
@@ -377,14 +408,14 @@ QED;
 (* for both kinds of links, linking preserve the ordering of the elements *)
 Theorem tree_link_order:
   !geq t1 t2.
-    WeakLinearOrder geq /\
+    TotalPreOrder geq /\
     is_tree_ordered geq t1 /\
     is_tree_ordered geq t2 ==>
     is_tree_ordered geq (tree_link geq t1 t2)
 Proof
   strip_tac \\
   ntac 2 Cases \\
-  rw[WeakLinearOrder, WeakOrder, tree_link_def,
+  rw[TotalPreOrder, PreOrder, tree_link_def,
      is_tree_ordered_def, BAG_EVERY, tree_to_bag_def]
   >- (Induct_on `l` \\
       rw[tree_to_bag_def, list_to_bag_def, is_tree_ordered_def, BAG_EVERY] \\
@@ -397,26 +428,26 @@ Proof
       fs[is_tree_ordered_def, BAG_EVERY] \\
       Induct_on `l'` \\
       rw[tree_to_bag_def, is_tree_ordered_def, BAG_EVERY] \\
-      metis_tac[transitive_def, reflexive_def,antisymmetric_def, trichotomous])
+      metis_tac[transitive_def, reflexive_def, total_def])
   >- (Induct_on `l` \\ rw[is_tree_ordered_def])
 QED;
 
 Theorem skew_link_order:
-  !geq x t1 t2. WeakLinearOrder geq /\
+  !geq x t1 t2. TotalPreOrder geq /\
                 is_tree_ordered geq t1 /\
                 is_tree_ordered geq t2 ==>
                 is_tree_ordered geq (skew_link geq x t1 t2)
 Proof
   ntac 2 strip_tac \\
   ntac 2 Cases \\
-  rw[WeakLinearOrder, WeakOrder, skew_link_def, tree_link_def,
+  rw[TotalPreOrder, PreOrder, skew_link_def, tree_link_def,
      is_tree_ordered_def, BAG_EVERY, tree_to_bag_def] \\
   fs[root_def, aux_def, children_def, rank_def] \\
   Induct_on `l` \\
   Induct_on `l'` \\
   rw[is_tree_ordered_def, BAG_EVERY, tree_to_bag_def, list_to_bag_def] \\
   fs[tree_to_bag_def, is_tree_ordered_def, BAG_EVERY] \\
-  metis_tac[transitive_def, reflexive_def, antisymmetric_def, trichotomous]
+  metis_tac[transitive_def, reflexive_def, total_def]
 QED;
 
 (*
@@ -435,7 +466,7 @@ Proof
 QED;
 
 Theorem binomial_insert_order:
-  !geq t h. WeakLinearOrder geq /\
+  !geq t h. TotalPreOrder geq /\
             is_heap_ordered geq h /\
             is_tree_ordered geq t ==>
             is_heap_ordered geq (binomial_insert geq t h)
@@ -468,7 +499,7 @@ Proof
 QED;
 
 Theorem insert_order:
-  !geq e h. WeakLinearOrder geq /\
+  !geq e h. TotalPreOrder geq /\
             is_heap_ordered geq h ==>
             is_heap_ordered geq (insert geq e h)
 Proof
@@ -482,7 +513,7 @@ Proof
 QED;
 
 Theorem insert_list_order:
-  !geq es h. WeakLinearOrder geq /\
+  !geq es h. TotalPreOrder geq /\
              is_heap_ordered geq h ==>
              is_heap_ordered geq (insert_list geq es h)
 Proof
@@ -530,7 +561,7 @@ Proof
 QED;
 
 Theorem normalize_order:
-  !geq h. WeakLinearOrder geq /\
+  !geq h. TotalPreOrder geq /\
           is_heap_ordered geq h ==>
           is_heap_ordered geq (normalize geq h)
 Proof
@@ -550,7 +581,7 @@ Proof
 QED;
 
 Theorem merge_tree_order:
-  !geq t1 t2. WeakLinearOrder geq /\
+  !geq t1 t2. TotalPreOrder geq /\
               is_heap_ordered geq t1 /\
               is_heap_ordered geq t2 ==>
               is_heap_ordered geq (merge_tree geq t1 t2)
@@ -580,7 +611,7 @@ Proof
 QED;
 
 Theorem merge_order:
-  !geq h1 h2. WeakLinearOrder geq /\
+  !geq h1 h2. TotalPreOrder geq /\
               is_heap_ordered geq h1 /\
               is_heap_ordered geq h2 ==>
               is_heap_ordered geq (merge geq h1 h2)
@@ -615,7 +646,7 @@ Proof
 QED;
 
 Theorem find_min_bag:
-  !geq h. WeakLinearOrder geq /\
+  !geq h. TotalPreOrder geq /\
           h <> [] /\
 	  is_heap_ordered geq h ==>
           BAG_IN (THE (find_min geq h)) (heap_to_bag h)
@@ -640,7 +671,7 @@ Proof
 QED;
 
 Theorem find_min_correct:
-  !geq h. WeakLinearOrder geq /\
+  !geq h. TotalPreOrder geq /\
           h <> [] /\
 	  is_heap_ordered geq h ==>
           !y. (BAG_IN y (heap_to_bag h)) ==> (geq y (THE (find_min geq h)))
@@ -654,7 +685,7 @@ Proof
           Induct_on `l`
           >- (rw[is_heap_ordered_def, heap_to_bag_def, find_min_def,
 		THE_DEF, root_def, tree_to_bag_def, is_tree_ordered_def] \\
-              fs[WeakLinearOrder, WeakOrder, reflexive_def, BAG_EVERY])
+              fs[TotalPreOrder, PreOrder, reflexive_def, BAG_EVERY])
 	  >- (rw[is_heap_ordered_def, heap_to_bag_def, find_min_def,
 		THE_DEF, root_def, tree_to_bag_def, is_tree_ordered_def,
 	        BAG_EVERY] \\
@@ -667,20 +698,20 @@ Proof
 	      >- (fs[heap_to_bag_def, is_heap_ordered_def]
 	          >- metis_tac[root_smallest]
 		  >- (res_tac \\ `geq y (THE (SOME x))` by metis_tac[] \\
-                      fs[THE_DEF, WeakOrder, WeakLinearOrder] \\
+                      fs[THE_DEF, PreOrder, TotalPreOrder] \\
                       metis_tac[transitive_def])
 		  >- (res_tac \\ `geq y (THE (SOME x))` by metis_tac[] \\
-                      fs[THE_DEF, WeakOrder, WeakLinearOrder] \\
+                      fs[THE_DEF, PreOrder, TotalPreOrder] \\
                       metis_tac[transitive_def]))
 	      >- (fs[heap_to_bag_def, is_heap_ordered_def]
 		  >- (`geq y (root h')` by rw[root_smallest] \\
-                      fs[WeakOrder, WeakLinearOrder] \\
-                      metis_tac[transitive_def, trichotomous])
+                      fs[PreOrder, TotalPreOrder] \\
+                      metis_tac[transitive_def, total_def])
 		  >- (res_tac \\ `geq y (THE (SOME x))` by metis_tac[] \\
-                      fs[THE_DEF, WeakOrder, WeakLinearOrder] \\
+                      fs[THE_DEF, PreOrder, TotalPreOrder] \\
                       metis_tac[transitive_def])
 		  >- (res_tac \\ `geq y (THE (SOME x))` by metis_tac[] \\
-                      fs[THE_DEF, WeakOrder, WeakLinearOrder] \\
+                      fs[THE_DEF, PreOrder, TotalPreOrder] \\
                       metis_tac[transitive_def])))))
 QED;
 
@@ -712,7 +743,7 @@ Proof
 QED;
 
 Theorem get_min_order:
-  !geq h smallest rest. WeakLinearOrder geq /\
+  !geq h smallest rest. TotalPreOrder geq /\
                          h <> [] /\
                          is_heap_ordered geq h /\
                          (smallest, rest) = get_min geq h ==>
@@ -738,7 +769,7 @@ Proof
 QED;
 
 Theorem get_min_correct:
-  !geq h smallest rest. WeakLinearOrder geq /\
+  !geq h smallest rest. TotalPreOrder geq /\
                         h <> [] /\
                         is_heap_ordered geq h /\
                         (smallest,rest) = get_min geq h ==>
@@ -765,7 +796,7 @@ Proof
 QED;
 
 Theorem delete_min_order:
-  !geq h. WeakLinearOrder geq /\
+  !geq h. TotalPreOrder geq /\
            h <> [] /\
            is_heap_ordered geq h ==>
            is_heap_ordered geq (THE (delete_min geq h))
@@ -783,7 +814,7 @@ Proof
 QED;
 
 Theorem delete_min_correct:
-  !geq h. WeakLinearOrder geq /\
+  !geq h. TotalPreOrder geq /\
            h <> [] /\
            is_heap_ordered geq h ==>
 	   heap_to_bag h = BAG_UNION
@@ -878,8 +909,7 @@ Proof
 QED;
 
 Theorem skew_b_order:
-  !geq b t1 t2. WeakLinearOrder geq /\
-                is_b_heap_ordered2 geq t1 /\
+  !geq b t1 t2. is_b_heap_ordered2 geq t1 /\
                 is_b_heap_ordered2 geq t2 /\
                 is_b_heap_ordered geq b ==>
                 is_b_heap_ordered2 geq (skew_link (b_heap_comparison geq) b t1 t2)
@@ -894,8 +924,7 @@ Proof
 QED;
 
 Theorem insert_b_order:
-  !geq b h. WeakLinearOrder geq /\
-            is_b_heap_ordered1 geq h /\
+  !geq b h. is_b_heap_ordered1 geq h /\
             is_b_heap_ordered geq b ==>
             is_b_heap_ordered1 geq (insert (b_heap_comparison geq) b h)
 Proof
@@ -911,7 +940,7 @@ Proof
 QED;
 
 Theorem b_merge_order:
-!geq h1 h2. WeakLinearOrder geq /\
+  !geq h1 h2. TotalPreOrder geq /\
               is_b_heap_ordered geq h1 /\
               is_b_heap_ordered geq h2 ==>
               is_b_heap_ordered geq (b_merge geq h1 h2)
@@ -926,18 +955,27 @@ Proof
       >- (fs[b_heap_to_bag_def, is_b_heap_ordered_def, BAG_EVERY] \\
           rw[] \\
           res_tac \\
-          fs[WeakLinearOrder, WeakOrder] \\
-          metis_tac[transitive_def, reflexive_def, trichotomous])
+          fs[TotalPreOrder, PreOrder] \\
+          metis_tac[transitive_def, reflexive_def, total_def])
       >- (fs[is_b_heap_ordered_def, BAG_EVERY])
+      >- (fs[is_b_heap_ordered_def] \\
+          imp_res_tac b_comparison_total_pre_order \\
+          imp_res_tac insert_order \\
+          rw[insert_b_order])
       >- (`is_b_heap_ordered1 geq l'` by fs[is_b_heap_ordered_def] \\
-          imp_res_tac insert_b_order))
+          imp_res_tac insert_b_order \\
+          rw[]))
     >- (rw[is_b_heap_ordered_def, b_bag_of_insert]
       >- (fs[b_heap_to_bag_def, is_b_heap_ordered_def, BAG_EVERY] \\
           rw[] \\
           res_tac \\
-          fs[WeakLinearOrder, WeakOrder] \\
-          metis_tac[transitive_def, reflexive_def, trichotomous])
+          fs[TotalPreOrder, PreOrder] \\
+          metis_tac[transitive_def, reflexive_def, total_def])
       >- (fs[is_b_heap_ordered_def, BAG_EVERY])
+      >- (fs[is_b_heap_ordered_def] \\
+          imp_res_tac insert_order \\
+          imp_res_tac b_comparison_total_pre_order \\
+          rw[insert_b_order])
       >- (`is_b_heap_ordered1 geq l` by fs[is_b_heap_ordered_def] \\
           imp_res_tac insert_b_order)))
 QED;
@@ -950,14 +988,14 @@ Proof
 QED;
 
 Theorem b_insert_order:
-  !geq e h. WeakLinearOrder geq /\
+  !geq e h. TotalPreOrder geq /\
             is_b_heap_ordered geq h ==>
             is_b_heap_ordered geq (b_insert geq e h)
 Proof
   rw[b_insert_def] \\
-  `is_b_heap_ordered geq (Bsbheap e [])`
-  by rw[is_b_heap_ordered_def, BAG_EVERY, b_heap_to_bag_def] \\
-  imp_res_tac b_merge_order
+  sg `is_b_heap_ordered geq (Bsbheap e [])`
+  >- rw[is_b_heap_ordered_def, is_heap_ordered_def, BAG_EVERY, b_heap_to_bag_def]
+  >- imp_res_tac b_merge_order
 QED;
 
 (* functional correctness of finding minimal element *)
@@ -971,7 +1009,7 @@ Proof
 QED;
 
 Theorem b_find_min_correct:
-  !geq h. WeakLinearOrder geq /\
+  !geq h. TotalPreOrder geq /\
           h <> Bsbempty /\
           is_b_heap_ordered geq h ==>
           BAG_EVERY (\y. geq y (THE (b_find_min h))) (b_heap_to_bag geq h)
@@ -982,7 +1020,7 @@ Proof
   >- rw[]
   >- (rw[b_find_min_def, THE_DEF] \\
       fs[is_b_heap_ordered_def, BAG_EVERY, b_heap_to_bag_def,
-	 WeakLinearOrder, WeakOrder] \\
+	 TotalPreOrder, PreOrder] \\
       metis_tac[reflexive_def])
 QED;
 
